floyd/forward.v
@@ -2,6 +2,7 @@ Require Import VST.floyd.base2.
 Require Import VST.floyd.client_lemmas.
 Require Import VST.floyd.go_lower.
 Require Import VST.floyd.closed_lemmas.
+Require Import VST.floyd.subsume_funspec.
 Require Import VST.floyd.forward_lemmas VST.floyd.call_lemmas.
 Require Import VST.floyd.extcall_lemmas.
 Require Import VST.floyd.nested_field_lemmas.
@@ -636,7 +637,7 @@ cbv beta iota zeta; unfold_post; extensionality rho;
 *)
 Ltac  forward_call_id1_wow := 
 let H := fresh in intro H;
-eapply (semax_call_id1_wow _ _ _ _ _ _ _ _ _ _ _ _ _ _ _ _ _ _ _ _ _ _ _ _ _ _ _ _ H); 
+eapply (semax_call_id1_wow _ _ _ _ _ _ _ _ _ _ _ _ _ _ _ _ _ _ _ _ _ _ _ _ _ _ _ _ _ H); 
  clear H; 
  lazymatch goal with Frame := _ : list mpred |- _ => try clear Frame end;
  [check_result_type
@@ -649,7 +650,10 @@ eapply (semax_call_id1_wow _ _ _ _ _ _ _ _ _ _ _ _ _ _ _ _ _ _ _ _ _ _ _ _ _ _ _
 
 Ltac forward_call_id1_x_wow :=
 let H := fresh in intro H;
-eapply (semax_call_id1_x_wow _ _ _ _ _ _ _ _ _ _ _ _ _ _ _ _ _ _ _ _ _ _ _ _ _ _ _ _ H); 
+eapply (semax_call_id1_x_wow 
+             _ _ _ _ _ _ _ _ _ _
+             _ _ _ _ _ _ _ _ _ _ 
+             _ _ _ _ _ _ _ _ _ H); 
  clear H;
  lazymatch goal with Frame := _ : list mpred |- _ => try clear Frame end;
  [ check_result_type | check_result_type
@@ -664,7 +668,10 @@ eapply (semax_call_id1_x_wow _ _ _ _ _ _ _ _ _ _ _ _ _ _ _ _ _ _ _ _ _ _ _ _ _ _
 
 Ltac forward_call_id1_y_wow :=
 let H := fresh in intro H;
-eapply (semax_call_id1_y_wow _ _ _ _ _ _ _ _ _ _ _ _ _ _ _ _ _ _ _ _ _ _ _ _ _ _ _ _ H); 
+eapply (semax_call_id1_y_wow 
+             _ _ _ _ _ _ _ _ _ _
+             _ _ _ _ _ _ _ _ _ _ 
+             _ _ _ _ _ _ _ _ _ H); 
  clear H;
  lazymatch goal with Frame := _ : list mpred |- _ => try clear Frame end;
  [ check_result_type | check_result_type
@@ -679,7 +686,7 @@ eapply (semax_call_id1_y_wow _ _ _ _ _ _ _ _ _ _ _ _ _ _ _ _ _ _ _ _ _ _ _ _ _ _
 
 Ltac forward_call_id01_wow :=
 let H := fresh in intro H;
-eapply (semax_call_id01_wow _ _ _ _ _ _ _ _ _ _ _ _ _ _ _ _ _ _ _ _ _ _ _ _ _ _ _ _ H); 
+eapply (semax_call_id01_wow _ _ _ _ _ _ _ _ _ _ _ _ _ _ _ _ _ _ _ _ _ _ _ _ _ _ _ _ _ H); 
  clear H;
  lazymatch goal with Frame := _ : list mpred |- _ => try clear Frame end;
  [ apply Coq.Init.Logic.I 
@@ -690,7 +697,7 @@ eapply (semax_call_id01_wow _ _ _ _ _ _ _ _ _ _ _ _ _ _ _ _ _ _ _ _ _ _ _ _ _ _ 
 
 Ltac forward_call_id00_wow  :=
 let H := fresh in intro H;
-eapply (semax_call_id00_wow _ _ _ _ _ _ _ _ _ _ _ _ _ _ _ _ _ _ _ _ _ _ _ _ _ _ _ _ H); 
+eapply (semax_call_id00_wow _ _ _ _ _ _ _ _ _ _ _ _ _ _ _ _ _ _ _ _ _ _ _ _ _ _ _ _ _ H); 
  clear H;
  lazymatch goal with Frame := _ : list mpred |- _ => try clear Frame end;
  [ check_result_type 
@@ -860,7 +867,7 @@ Proof.
 intros. constructor.
 Qed.
 
-Ltac prove_call_setup1 :=
+Ltac prove_call_setup1 subsumes :=
 match goal with |- @semax ?CS _ ?Delta (PROPx ?P (LOCALx ?Q (SEPx ?R))) ?c _ =>
  lazymatch c with
  | context [Scall _ (Evar ?id ?ty) ?bl] =>
@@ -873,6 +880,7 @@ match goal with |- @semax ?CS _ ?Delta (PROPx ?P (LOCALx ?Q (SEPx ?R))) ?c _ =>
       | find_spec_in_globals'
       | simpl; reflexivity  (* function-id type in AST matches type in funspec *)
       ]
+    | apply subsumes
     | auto 50 with derives
     | simpl; reflexivity  (* function-id type in AST matches type in funspec *)
     |check_typecheck
@@ -887,6 +895,7 @@ match goal with |- @semax ?CS _ ?Delta (PROPx ?P (LOCALx ?Q (SEPx ?R))) ?c _ =>
  [check_prove_local2ptree
  |reflexivity
  |prove_func_ptr
+ | apply subsumes
  |auto 50 with derives
  |check_parameter_types
  |check_typecheck
@@ -897,17 +906,17 @@ match goal with |- @semax ?CS _ ?Delta (PROPx ?P (LOCALx ?Q (SEPx ?R))) ?c _ =>
  end
 end.
 
-Ltac prove_call_setup witness :=
- prove_call_setup1;
+Ltac prove_call_setup subsumes witness :=
+ prove_call_setup1 subsumes;
  [ .. | 
- match goal with |- call_setup1 _ _ _ _ _ _ _ _ _ _ _ _ _ ?A _ _ _ _ _ _ _ -> _ =>
+ match goal with |- call_setup1 _ _ _ _ _ _ _ _ _ _ _ _ _ _ ?A _ _ _ _ _ _ _ -> _ =>
       check_witness_type A witness
  end;
  let H := fresh in
  intro H;
  match goal with | |- @semax ?CS _ _ _ _ _ =>
  let Frame := fresh "Frame" in evar (Frame: list mpred);
- exploit (call_setup2_i _ _ _ _ _ _ _ _ _ _ _ _ _ _ _ _ _ _ _ _ _ H witness Frame); clear H;
+ exploit (call_setup2_i _ _ _ _ _ _ _ _ _ _ _ _ _ _ _ _ _ _ _ _ _ _ H witness Frame); clear H;
  [ reflexivity
  | check_prove_local2ptree
  | Forall_pTree_from_elements
@@ -917,17 +926,17 @@ Ltac prove_call_setup witness :=
  ]
  end].
 
-Ltac fwd_call' witness :=
+Ltac fwd_call' subsumes witness :=
 lazymatch goal with
 | |- semax _ _ (Ssequence (Scall _ _ _) _) _ =>
   eapply semax_seq';
-    [prove_call_setup witness;
+    [prove_call_setup subsumes witness;
      clear_Delta_specs; clear_MORE_POST;
      [ .. |
       lazymatch goal with
       | |- _ -> semax _ _ (Scall (Some _) _ _) _ =>
          forward_call_id1_wow
-      | |- call_setup2 _ _ _ _ _ _ _ _ _ _ _ ?retty _ _ _ _ _ _ _ _ _ _ _ _ _ _ _ _ ->
+      | |- call_setup2 _ _ _ _ _ _ _ _ _ _ _ _ ?retty _ _ _ _ _ _ _ _ _ _ _ _ _ _ _ _ ->
                 semax _ _ (Scall None _ _) _ =>
         tryif (unify retty Tvoid)
         then forward_call_id00_wow
@@ -938,7 +947,7 @@ lazymatch goal with
                                        (Sset _ (Ecast (Etempvar ?ret'2 _) _))) _) _ =>
        unify ret' ret'2;
        eapply semax_seq';
-         [prove_call_setup witness;
+         [prove_call_setup subsumes witness;
           clear_Delta_specs; clear_MORE_POST;
              [ .. | forward_call_id1_x_wow ]
          |  after_forward_call ]
@@ -946,15 +955,15 @@ lazymatch goal with
                                        (Sset _ (Etempvar ?ret'2 _))) _) _ =>
        unify ret' ret'2;
        eapply semax_seq';
-         [prove_call_setup witness;
+         [prove_call_setup subsumes witness;
           clear_Delta_specs; clear_MORE_POST;
              [ .. | forward_call_id1_y_wow ]
          |  after_forward_call ]
-| |- _ => rewrite <- seq_assoc; fwd_call' witness
+| |- _ => rewrite <- seq_assoc; fwd_call' subsumes witness
 end.
 
 
-Ltac fwd_call witness :=
+Ltac fwd_call subsumes witness :=
  try lazymatch goal with
       | |- semax _ _ (Scall _ _ _) _ => rewrite -> semax_seq_skip
       end;
@@ -964,11 +973,13 @@ Ltac fwd_call witness :=
  end;
 lazymatch goal with |- @semax ?CS _ ?Delta _ (Ssequence ?C _) _ =>
   lazymatch C with context [Scall _ _ _] =>
-         fwd_call' witness
+         fwd_call' subsumes witness
     end
 end.
 
-Tactic Notation "forward_call" constr(witness) := fwd_call witness.
+Tactic Notation "forward_call" constr(witness) := fwd_call subsume_funspec_refl witness.
+
+Tactic Notation "forward_call" constr(subsumes) constr(witness) := fwd_call subsumes witness.
 
 Lemma seq_assoc2:
   forall (Espec: OracleKind) {cs: compspecs}  Delta P c1 c2 c3 c4 Q,
